src/drf/PromiseConsistent.v
@@ -22,6 +22,8 @@ Require Import SimPromises.
 Require Import SimLocal.
 Require Import FulfillStep.
 Require Import MemoryReorder.
+Require Import Configuration.
+Require Import SmallStep.
 
 Set Implicit Arguments.
 
@@ -30,6 +32,11 @@ Definition promise_consistent (lc:Local.t): Prop :=
   forall loc ts from msg
     (PROMISE: Memory.get loc ts lc.(Local.promises) = Some (from, msg)),
     Time.lt (lc.(Local.commit).(Commit.cur).(Capability.rw) loc) ts.
+
+Definition promise_consistent_th (tid: Ident.t) (c: Configuration.t) : Prop :=
+  forall lst lc
+         (THREAD: IdentMap.find tid c.(Configuration.threads) = Some (lst, lc)),
+  promise_consistent lc.
 
 Lemma promise_step_promise_consistent
       lc1 mem1 loc from to val released lc2 mem2 kind
@@ -180,3 +187,124 @@ Proof.
     exploit Memory.promise_promises_get1; eauto. i. des.
     exploit fulfill_unset_promises; eauto. i. des. subst. refl.
 Qed.  
+
+Lemma thread_step_unset_promises
+      lang loc e from ts msg (th1 th2:Thread.t lang)
+      (STEP: Thread.step e th1 th2)
+      (TH1: Memory.get loc ts th1.(Thread.local).(Local.promises) = Some (from, msg))
+      (TH2: Memory.get loc ts th2.(Thread.local).(Local.promises) = None):
+  exists ord from val rel,
+  <<EVENT: ThreadEvent.is_writing e = Some (loc, from, ts, val, rel, ord)>> /\
+  <<ORD: Ordering.le ord Ordering.relaxed>> /\
+  <<TIME: Time.lt (th1.(Thread.local).(Local.commit).(Commit.cur).(Capability.rw) loc) ts>>.
+Proof.
+  inv STEP.
+  { inv STEP0. inv LOCAL. destruct msg. ss. 
+    exploit Memory.promise_promises_get1; eauto. i. des. congr.
+  }
+  destruct msg.
+  inv STEP0; ss; try by inv LOCAL; ss; congr.
+  - by rewrite TH1 in TH2.
+  - inv LOCAL. inv WRITE.
+    exploit Memory.promise_promises_get1; eauto. i. des.
+    exploit fulfill_unset_promises; eauto. i. des. subst.
+    unfold Memory.get in *.
+    esplits; s; eauto.
+    + edestruct ordering_relaxed_dec; eauto.
+      apply RELEASE in H. des. ss. by rewrite H, Cell.bot_get in TH1.
+    + inv WRITABLE. eauto.
+  - inv LOCAL1. inv LOCAL2. inv WRITE.
+    exploit Memory.promise_promises_get1; eauto. i. des.
+    exploit fulfill_unset_promises; eauto. i. des. subst.
+    unfold Memory.get in *.
+    esplits; s; eauto.
+    + edestruct ordering_relaxed_dec; eauto.
+      apply RELEASE in H. des. ss. by rewrite H, Cell.bot_get in TH1.
+    + inv WRITABLE. inv READABLE. ss. move TS at bottom.
+      eapply TimeFacts.le_lt_lt; eauto.
+      repeat (etrans; [|apply Time.join_l]). refl.
+Qed.
+
+Lemma rtc_small_step_unset_promises
+      tid loc ts c1 lst1 lc1 c2 lst2 lc2 from msg withprm
+      (STEPS: rtc (small_step_evt withprm tid) c1 c2)
+      (WF: Configuration.wf c1)
+      (FIND1: IdentMap.find tid c1.(Configuration.threads) = Some (lst1, lc1))
+      (GET1: Memory.get loc ts lc1.(Local.promises) = Some (from, msg))
+      (FIND2: IdentMap.find tid c2.(Configuration.threads) = Some (lst2, lc2))
+      (GET2: Memory.get loc ts lc2.(Local.promises) = None):
+  Time.lt (lc1.(Local.commit).(Commit.cur).(Capability.rw) loc) ts.
+Proof.
+  ginduction STEPS; i; subst.
+  { ss. rewrite FIND1 in FIND2. depdes FIND2.
+    by rewrite GET1 in GET2.
+  }
+  inv H. 
+  exploit small_step_future; eauto. intros [WF2 _].
+  inv USTEP. ss. rewrite FIND1 in TID. depdes TID.
+  destruct (Memory.get loc ts lc3.(Local.promises)) as [[t m]|] eqn: PRM.
+  - rewrite IdentMap.gss in IHSTEPS.
+    exploit IHSTEPS; eauto.
+    intro LT. move STEP at bottom.
+    eapply TimeFacts.le_lt_lt; eauto.
+    inv WF. exploit thread_step_commit_le; try exact STEP; eauto. 
+    { eapply WF0. rewrite FIND1. eauto. }
+    s. i. apply x1.
+  - eapply thread_step_unset_promises in STEP; eauto. des.
+    eauto using small_step_write_lt.
+Qed.
+
+Lemma promise_consistent_th_small_step
+      tid c1 c2 withprm
+      (STEP: small_step_evt withprm tid c1 c2)
+      (WF: Configuration.wf c1)
+      (FULFILL: promise_consistent_th tid c2):
+  promise_consistent_th tid c1.
+Proof.
+  ii. destruct (IdentMap.find tid (Configuration.threads c2)) as [[lang2 lc2]|] eqn: THREAD2; cycle 1.
+  { inv STEP. inv USTEP. ss. by rewrite IdentMap.gss in THREAD2. }
+  destruct (Memory.get loc ts (Local.promises lc2)) as [[from2 msg2]|] eqn: PROMISE2; cycle 1.
+  - apply Operators_Properties.clos_rt1n_step in STEP.
+    eapply rtc_small_step_unset_promises; eauto.
+  - eapply FULFILL in PROMISE2; eauto.
+    eapply TimeFacts.le_lt_lt; eauto.
+    inv STEP. inv USTEP. ss.
+    rewrite THREAD in TID. inv TID.
+    rewrite IdentMap.gss in THREAD2. inv THREAD2.
+    inv WF. exploit thread_step_commit_le; try exact STEP; eauto. 
+    { eapply WF0. rewrite THREAD. eauto. }
+    s. i. apply x0.
+Qed.
+
+Lemma promise_consistent_th_rtc_small_step
+      tid c1 c2 withprm
+      (STEP: rtc (small_step_evt withprm tid) c1 c2)
+      (WF: Configuration.wf c1)
+      (FULFILL: promise_consistent_th tid c2):
+  promise_consistent_th tid c1.
+Proof.
+  ginduction STEP; eauto. 
+  i. eapply promise_consistent_th_small_step; eauto.
+  eapply IHSTEP; eauto.
+  inv H. eapply small_step_future; eauto.
+Qed.
+
+Lemma consistent_promise_consistent_th
+      tid c 
+      (WF: Configuration.wf c)
+      (CONSISTENT: Configuration.consistent c):
+  promise_consistent_th tid c.
+Proof.
+  ii. assert (X:= WF). inv X. inv WF0. destruct lst as [lang st].
+  exploit CONSISTENT; eauto; try reflexivity.
+  i; des. destruct e2.
+  exploit rtc_thread_step_rtc_small_step; [eauto|..].
+  { ss. eapply rtc_implies, STEPS. i; inv PR; eauto. }
+  intro STEPS2. 
+  eapply rtc_small_step_unset_promises in STEPS2; eauto.
+  - destruct c. eapply rtc_small_step_future; eauto.
+  - s. rewrite IdentMap.gss. eauto.
+  - ss. rewrite PROMISES. apply Cell.bot_get.
+Grab Existential Variables. exact true.
+Qed.
+
